VisualProof/Diagram/Concrete/WireQuantifierRelationJoinAlignment.lean
@@ -1,6 +1,4 @@
-import VisualProof.Diagram.Concrete.WireQuantifierSemantics
 import VisualProof.Diagram.Concrete.WireQuantifierRelationJoin
-import VisualProof.Diagram.Concrete.WireQuantifierExhaustedWireRemoval
 import VisualProof.Diagram.Concrete.WireQuantifierSingletonRemovalZipper
 import VisualProof.Diagram.Concrete.Subgraph.FactorizationNaturalityZipper
 
